dev/lf/tight-proof/Inert_types.v
@@ -4,29 +4,54 @@ Require Import LibLN.
 Require Import Coq.Program.Equality.
 Require Import Definitions.
 Require Import Some_lemmas.
-Require Import Precise_flow.
+
+(*
+Definition (Precise flow of a variable)
+If G(x)=T, then T is in Pf(x,G,T).
+If rec(x:U) is in Pf(x,G,T), then U is in Pf(x,G,T).
+If (U1 & U2) is in Pf(x,G,T), then U1 is in Pf(x,G,T).
+If (U1 & U2) is in Pf(x,G,T), then U2 is in Pf(x,G,T). *)
+
+Inductive precise_flow : var -> ctx -> typ -> typ -> Prop :=
+  | pf_bind : forall x G T,
+      binds x T G ->
+      precise_flow x G T T
+  | pf_open : forall x G T U,
+      precise_flow x G T (typ_bnd U) ->
+      precise_flow x G T (open_typ x U)
+  | pf_and1 : forall x G T U1 U2,
+      precise_flow x G T (typ_and U1 U2) ->
+      precise_flow x G T U1
+  | pf_and2 : forall x G T U1 U2,
+      precise_flow x G T (typ_and U1 U2) ->
+      precise_flow x G T U2.
+
+Hint Constructors precise_flow.
+
+Lemma precise_flow_lemma : forall U G x,
+    ty_trm ty_precise sub_general G (trm_var (avar_f x)) U ->
+    exists T, precise_flow x G T U.
+Proof.
+  introv H. dependent induction H; try (destruct* (IHty_trm _ eq_refl eq_refl eq_refl)); eauto.
+Qed.
+
+Lemma precise_flow_all_inv : forall p G S T U,
+    precise_flow p G (typ_all S T) U ->
+    U = typ_all S T.
+Proof.
+  introv Hpf.
+  dependent induction Hpf; auto;
+    specialize (IHHpf S T eq_refl); inversion IHHpf.
+Qed.
 
 (* ###################################################################### *)
 (** ** Inert types *)
-
-(* Definition (Inert types)
-
-A type is inert if it of the form
-  all(x: S)T
-  rec(x: T), where T is a record type
- *)
 
 Inductive inert_typ : typ -> Prop :=
   | inert_typ_all : forall S T, inert_typ (typ_all S T) (* all(x: S)T *)
   | inert_typ_bnd : forall T,
       record_type T ->
       inert_typ (typ_bnd T). (* rec(x:T) *)
-
-(* Definition (Inert context)
-
-A context is inert if it is of the form
-  {}
-  G, x : T where G is a inert context and T is a inert type *)
 
 Inductive inert : ctx -> Prop :=
   | inert_empty : inert empty
@@ -35,9 +60,6 @@ Inductive inert : ctx -> Prop :=
       inert_typ T ->
       x # pre ->
       inert (pre & x ~ T).
-
-(* Inert contexts bind inert:
-If G |- x : T and G is a inert context then T is a inert type. *)
 
 Lemma binds_inert : forall G x T,
     binds x T G ->
@@ -51,147 +73,314 @@ Proof.
     + destruct H1. apply (IHHinert H2).
 Qed.
 
-Lemma inert_binds : forall G x T,
-    inert G ->
-    binds x T G ->
-    inert_typ T.
-Proof.
-  introv Bi Hgd.
-  eapply binds_inert; eauto.
-Qed.
-
 Lemma inert_typ_bnd_record : forall G x T,
     inert G ->
     binds x (typ_bnd T) G ->
     record_type T.
 Proof.
   introv Bi Hgd.
-  pose proof (inert_binds Bi Hgd).
+  pose proof (binds_inert Hgd Bi).
   dependent induction H.
   assumption.
 Qed.
 
-Lemma inert_unique_tight_bounds' : forall G x T T1 T2 A,
-    inert_typ T ->
-    precise_flow x G T (typ_rcd (dec_typ A T1 T1)) ->
-    precise_flow x G T (typ_rcd (dec_typ A T2 T2)) ->
-    T1 = T2.
-Proof.
-  introv Hgt Hpf1 Hpf2.
-  induction Hgt.
-  - apply precise_flow_all_inv in Hpf1.
-    inversion Hpf1.
-  - apply (record_unique_tight_bounds H Hpf1 Hpf2).
-Qed.
-
-Lemma inert_unique_tight_bounds: forall G x T1 T2 A,
-  inert G ->
-  ty_trm ty_precise sub_general G (trm_var (avar_f x)) (typ_rcd (dec_typ A T1 T1)) ->
-  ty_trm ty_precise sub_general G (trm_var (avar_f x)) (typ_rcd (dec_typ A T2 T2)) ->
-  T1 = T2.
-Proof.
-  introv Hgd Hty1 Hty2.
-  assert (exists T, binds x T G) as Bi. {
-    eapply typing_implies_bound. eassumption.
-  }
-  destruct Bi as [T Bi].
-  pose proof (inert_binds Hgd Bi) as Hgt.
-  pose proof (precise_flow_lemma Bi Hty1) as H1.
-  pose proof (precise_flow_lemma Bi Hty2) as H2.
-  apply (inert_unique_tight_bounds' Hgt H1 H2).
-Qed.
-
-Lemma inert_precise_bot : forall T G x,
+Lemma pf_inert_T : forall G p T U,
     inert G ->
-    binds x T G ->
+    precise_flow p G T U ->
+    inert_typ T.
+Proof.
+  introv Hi Pf. induction Pf; eauto.
+  apply (binds_inert H Hi).
+Qed.
+
+Lemma pf_rcd_T : forall G p T U,
+    inert G ->
+    precise_flow p G (typ_bnd T) U ->
+    record_type T.
+Proof.
+  introv Hi Pf. apply pf_inert_T in Pf; inversions Pf; assumption.
+Qed.
+
+Lemma pf_inert_or_rcd : forall G x T U,
+    inert G ->
+    precise_flow x G (typ_bnd T) U ->
+    U = typ_bnd T \/ record_type U.
+Proof.
+  introv Hi Pf.
+  dependent induction Pf; try solve [left*].
+  - specialize (IHPf T Hi eq_refl). destruct IHPf as [eq | r].
+    * inversions eq. right. lets Hr: (pf_rcd_T Hi Pf). apply* open_record_type.
+    * inversion r. inversion H.
+  - right. destruct (IHPf T Hi eq_refl) as [F | Hr]. inversion F. inversion Hr. inversions H.
+    exists ls. assumption.
+  - right. destruct (IHPf T Hi eq_refl) as [F | Hr]. inversion F. inversion Hr. inversions H.
+    eexists. apply* rt_one.
+Qed.
+
+Lemma pf_inert_lambda_T : forall G x T U S,
+    inert G ->
+    precise_flow x G (typ_all T U) S ->
+    S = typ_all T U.
+Proof.
+  introv Hi Pf. dependent induction Pf;
+                  try (specialize (IHPf T U Hi eq_refl); inversion IHPf); auto.
+Qed.
+
+Lemma pf_inert_bnd_U: forall G x T U,
+    inert G ->
+    precise_flow x G T (typ_bnd U) ->
+    T = typ_bnd U.
+Proof.
+  introv Hi Pf.
+  lets HT: (pf_inert_T Hi Pf). inversions HT; dependent induction Pf; auto.
+  - destruct U0; inversions x.
+    apply pf_inert_lambda_T in Pf. inversion* Pf. assumption.
+  - apply pf_inert_lambda_T in Pf. inversion Pf. assumption.
+  - apply pf_inert_lambda_T in Pf. inversion Pf. assumption.
+  - specialize (IHPf U0 Hi T0 eq_refl eq_refl H).
+    destruct (pf_inert_or_rcd Hi Pf) as [Heq | Hr].
+    * inversions Heq. destruct T0; inversions x. inversion H. inversion H0.
+    * inversions IHPf. inversion Hr. inversions H0.
+  - destruct (pf_inert_or_rcd Hi Pf) as [Heq | Hr].
+    * inversions Heq.
+    * inversions Hr. inversions H0. inversions H3.
+  - destruct (pf_inert_or_rcd Hi Pf) as [Heq | Hr].
+    * inversions Heq.
+    * inversions Hr. inversions H0.
+Qed.
+
+Lemma pf_inert_rcd_U: forall G x T D,
+    inert G ->
+    precise_flow x G T (typ_rcd D) ->
+    exists U, T = typ_bnd U.
+Proof.
+  introv Hi Pf.
+  lets HT: (pf_inert_T Hi Pf). inversions HT; dependent induction Pf; auto.
+  - apply (pf_inert_lambda_T Hi) in Pf. inversion Pf.
+  - apply (pf_inert_lambda_T Hi) in Pf. inversion Pf.
+  - apply pf_inert_lambda_T in Pf. inversion Pf. assumption.
+  - apply (pf_inert_bnd_U Hi) in Pf. exists* U.
+  - exists* T0.
+  - exists* T0.
+Qed.
+
+Lemma pf_inert_rcd_typ_U: forall G x T Ds,
+    inert G ->
+    precise_flow x G T Ds ->
+    record_type Ds ->
+    exists U, T = typ_bnd U.
+Proof.
+  introv Hi Pf Hr.
+  lets HT: (pf_inert_T Hi Pf). inversions HT; dependent induction Pf; auto.
+  - inversion Hr. inversion H0.
+  - apply (pf_inert_lambda_T Hi) in Pf. inversion Pf.
+  - apply (pf_inert_lambda_T Hi) in Pf. inversion Pf.
+  - apply pf_inert_lambda_T in Pf. inversion Pf. assumption.
+  - inversion Hr. inversion H1.
+  - apply (pf_inert_bnd_U Hi) in Pf. exists* U.
+  - apply* IHPf. destruct (pf_inert_or_rcd Hi Pf) as [H1 | H1]. inversion H1. assumption.
+  - apply* IHPf. destruct (pf_inert_or_rcd Hi Pf) as [H1 | H1]. inversion H1. assumption.
+Qed.
+
+Lemma pf_inert_rcd_bnd_U : forall G x T U,
+    inert G ->
+    precise_flow x G T (typ_bnd U) ->
+    record_type U.
+Proof.
+  introv Hi Pf. lets HT: (pf_inert_bnd_U Hi Pf). subst.
+  lets HiT: (pf_rcd_T Hi Pf). assumption.
+Qed.
+
+Lemma pf_inert_lambda_U : forall x G S T U,
+    inert G ->
+    precise_flow x G U (typ_all S T) ->
+    U = typ_all S T.
+Proof.
+  introv Hi Pf.
+  lets Hiu: (pf_inert_T Hi Pf).
+  inversions Hiu.
+  - apply (pf_inert_lambda_T Hi) in Pf. inversion* Pf.
+  - destruct (pf_inert_or_rcd Hi Pf) as [H1 | H1]; inversions H1. inversion H0.
+Qed.
+
+Lemma pf_bot_false : forall G x T,
+    inert G ->
     precise_flow x G T typ_bot ->
     False.
 Proof.
-  intros T G x Hgd Bis Hpf.
-  pose proof (binds_inert Bis Hgd) as Hgtyp.
-  induction Hgtyp.
-  - apply precise_flow_all_inv in Hpf.
-    inversion Hpf.
-  - pose proof (precise_flow_bnd_eq_or_record H Hpf) as [[U [Contra _]] | [? Contra]];
-      inversion Contra.
+  introv Hi Pf.
+  lets HT: (pf_inert_T Hi Pf). inversions HT.
+  - apply (pf_inert_lambda_T Hi) in Pf. inversion Pf.
+  - destruct (pf_inert_or_rcd Hi Pf); inversion H0. inversion H1.
 Qed.
 
-Lemma inert_ty_precise_bot : forall G x,
+Lemma precise_bot_false : forall G x,
     inert G ->
     ty_trm ty_precise sub_general G (trm_var (avar_f x)) typ_bot ->
     False.
 Proof.
-  intros G x Hgd Hpt.
-  pose proof (typing_implies_bound Hpt) as [T Bi].
-  pose proof (precise_flow_lemma Bi Hpt) as Hpf.
-  eapply inert_precise_bot; eassumption.
+  introv Hi Hp. destruct (precise_flow_lemma Hp) as [T Pf].
+  apply* pf_bot_false.
 Qed.
 
-Lemma inert_precise_sel_inv : forall G x y A,
+Lemma pf_psel_false : forall G T x y A,
+    inert G ->
+    precise_flow x G T (typ_sel y A) ->
+    False.
+Proof.
+  introv Hi Pf.
+  lets HT: (pf_inert_T Hi Pf). inversions HT.
+  - apply (pf_inert_lambda_T Hi) in Pf. inversion Pf.
+  - destruct (pf_inert_or_rcd Hi Pf); inversion H0. inversion H1.
+Qed.
+
+Lemma precise_psel_false : forall G x y A,
     inert G ->
     ty_trm ty_precise sub_general G (trm_var (avar_f x)) (typ_sel y A) ->
     False.
 Proof.
-  introv Hgd Hpt.
-  pose proof (typing_implies_bound Hpt) as [T Bis].
-  pose proof (inert_binds Hgd Bis) as Hgt.
-  pose proof (precise_flow_lemma Bis Hpt) as Hpf.
-  induction Hgt.
-  - apply (precise_flow_all_inv) in Hpf.
-    inversion Hpf.
-  - pose proof (precise_flow_bnd_eq_or_record H Hpf) as [[U [Contra H1]] | [ls Contra]]; inversion Contra.
+  introv Hi Hp. destruct (precise_flow_lemma Hp) as [T Pf].
+  apply* pf_psel_false.
 Qed.
 
-Lemma inert_precise_dec_implies_record_dec : forall G x D,
+Lemma pf_record_sub : forall x G T T' D,
     inert G ->
-    ty_trm ty_precise sub_general G (trm_var (avar_f x)) (typ_rcd D) ->
-    record_dec D.
+    precise_flow x G (typ_bnd T) T' ->
+    record_has T' D ->
+    record_has (open_typ x T) D.
 Proof.
-  introv Hgd Hpt.
-  pose proof (typing_implies_bound Hpt) as [T' Bis].
-  pose proof (inert_binds Hgd Bis) as Hgt.
-  pose proof (precise_flow_lemma Bis Hpt) as Hpf.
-  induction Hgt.
-  - apply (precise_flow_all_inv) in Hpf.
-    inversion Hpf.
-  - apply (record_precise_dec_implies_record_dec H Hpf).
+  introv Hi Pf Hr. dependent induction Pf.
+  - inversions Hr.
+  - apply (pf_inert_bnd_U Hi) in Pf. inversion* Pf.
+  - apply* IHPf.
+  - apply* IHPf.
 Qed.
 
-Lemma inert_precise_dec_typ_inv : forall G x A S U,
+Lemma precise_flow_record_has: forall S G x D,
     inert G ->
-    ty_trm ty_precise sub_general G (trm_var (avar_f x)) (typ_rcd (dec_typ A S U)) ->
-    S = U.
+    precise_flow x G (typ_bnd S) (typ_rcd D) ->
+    record_has (open_typ x S) D.
 Proof.
-  introv Hgd Hpt.
-  pose proof (inert_precise_dec_implies_record_dec Hgd Hpt) as Hrec.
-  inversion Hrec.
-  reflexivity.
+  introv Hi Pf.
+  apply* pf_record_sub.
 Qed.
 
-Lemma inert_precise_flow_all_inv : forall x G S T U,
+Lemma pf_record_unique_tight_bounds_rec : forall G x T A T1 T2,
     inert G ->
-    precise_flow x G U (typ_all S T) ->
-    U = (typ_all S T).
+    precise_flow x G (typ_bnd T) (typ_rcd (dec_typ A T1 T1)) ->
+    precise_flow x G (typ_bnd T) (typ_rcd (dec_typ A T2 T2)) ->
+    T1 = T2.
 Proof.
-  introv Hgd Hpf.
-  pose proof (precise_flow_implies_bound Hpf) as Bis.
-  pose proof (inert_binds Hgd Bis) as Hgt.
-  dependent induction Hgt.
-  - symmetry. eapply precise_flow_all_inv. eassumption.
-  - pose proof (precise_flow_bnd_eq_or_record H Hpf) as [ [? [Contra _]] | [? Contra]]; inversion Contra.
+  introv Hi Pf1 Pf2.
+  pose proof (precise_flow_record_has Hi Pf1) as H1.
+  pose proof (precise_flow_record_has Hi Pf2) as H2.
+  eapply unique_rcd_typ; eauto. apply (pf_rcd_T Hi) in Pf1.
+  apply* open_record_type.
 Qed.
 
-Lemma inert_precise_all_inv : forall x G S T,
+Lemma pf_inert_unique_tight_bounds : forall G x T T1 T2 A,
     inert G ->
-    ty_trm ty_precise sub_general G (trm_var (avar_f x)) (typ_all S T) ->
-    binds x (typ_all S T) G.
+    precise_flow x G T (typ_rcd (dec_typ A T1 T1)) ->
+    precise_flow x G T (typ_rcd (dec_typ A T2 T2)) ->
+    T1 = T2.
 Proof.
-  introv Hgd Htyp.
-  pose proof (typing_implies_bound Htyp) as [U Bi].
-  pose proof (precise_flow_lemma Bi Htyp) as Hpf.
-  pose proof (inert_precise_flow_all_inv Hgd Hpf) as H.
-  rewrite <- H.
-  assumption.
+  introv Hi Pf1 Pf2.
+  assert (record_type (typ_rcd (dec_typ A T1 T1))) as Hrt. {
+    unfold record_type. eexists. apply* rt_one.
+    constructor.
+  }
+  lets Hr: (pf_inert_rcd_typ_U Hi Pf1 Hrt). destruct Hr as [U Heq]. subst.
+  apply* pf_record_unique_tight_bounds_rec.
+Qed.
+
+Lemma pf_binds: forall G x T U,
+    precise_flow x G T U ->
+    binds x T G.
+Proof.
+  introv Pf. dependent induction Pf; auto.
+Qed.
+
+Lemma inert_pt_unique: forall G x T T1 T2,
+    inert G ->
+    precise_flow x G T T1 ->
+    precise_flow x G T T2 ->
+    inert_typ T1 ->
+    inert_typ T2 ->
+    T1 = T2.
+Proof.
+  introv Hi P1 P2 I1 I2. inversions I1; inversions I2.
+  - apply (pf_inert_lambda_U Hi) in P1.
+    apply (pf_inert_lambda_U Hi) in P2. inversions* P2.
+  - apply (pf_inert_bnd_U Hi) in P2.
+    apply (pf_inert_lambda_U Hi) in P1. inversions* P2.
+  - apply (pf_inert_bnd_U Hi) in P1.
+    apply (pf_inert_lambda_U Hi) in P2. inversions* P2.
+  - apply (pf_inert_bnd_U Hi) in P2.
+    apply (pf_inert_bnd_U Hi) in P1. inversions* P2.
+Qed.
+
+Lemma pf_rcd_unique: forall G x T a U1 U2,
+    inert G ->
+    precise_flow x G T (typ_rcd (dec_trm a U1)) ->
+    precise_flow x G T (typ_rcd (dec_trm a U2 )) ->
+    U1 = U2.
+Proof.
+  introv Hi Pf1 Pf2. dependent induction Pf1.
+  - apply (binds_inert H) in Hi. inversion Hi.
+  - assert (record_type (typ_rcd (dec_trm a U2))) as Hrt. {
+      eexists. apply* rt_one. constructor.
+    }
+    destruct (pf_inert_rcd_typ_U Hi Pf2 Hrt) as [S Heq]. subst.
+    destruct U; inversions x. destruct d; inversions H0.
+    apply (pf_inert_bnd_U Hi) in Pf1. inversions Pf1.
+    lets Hr: (precise_flow_record_has Hi Pf2). inversion* Hr.
+  - assert (record_type (typ_rcd (dec_trm a U2))) as Hrt. {
+      eexists. apply* rt_one. constructor.
+    }
+    destruct (pf_inert_rcd_typ_U Hi Pf2 Hrt) as [S Heq]. subst.
+    assert (record_has (typ_and (typ_rcd (dec_trm a U1)) U0) (dec_trm a U1)) as H
+        by (apply* rh_andl).
+    lets Hr1: (pf_record_sub Hi Pf1 H).
+    lets Hr2: (precise_flow_record_has Hi Pf2).
+    assert (record_type (open_typ x S)) as Hs. {
+      apply open_record_type. apply pf_inert_T in Pf1. inversion* Pf1. assumption.
+    }
+    apply* unique_rcd_trm.
+  - assert (record_type (typ_rcd (dec_trm a U2))) as Hrt. {
+      eexists. apply* rt_one. constructor.
+    }
+    destruct (pf_inert_rcd_typ_U Hi Pf2 Hrt) as [S Heq]. subst.
+    assert (record_has (typ_and U3 (typ_rcd (dec_trm a U1))) (dec_trm a U1)) as H
+        by (apply* rh_andr).
+    lets Hr1: (pf_record_sub Hi Pf1 H).
+    lets Hr2: (precise_flow_record_has Hi Pf2).
+    assert (record_type (open_typ x S)) as Hs. {
+      apply open_record_type. apply pf_inert_T in Pf1. inversion* Pf1. assumption.
+    }
+    apply* unique_rcd_trm.
+Qed.
+
+Lemma x_bound_unique: forall G x T1 T2 U1 U2,
+    inert G ->
+    precise_flow x G T1 U1 ->
+    precise_flow x G T2 U2 ->
+    T1 = T2.
+Proof.
+  introv Hi Pf1. gen T2 U2. induction Pf1; intros; try solve [apply* IHPf1]; auto.
+  apply pf_binds in H0. apply (binds_func H H0).
+Qed.
+
+Lemma inert_unique_tight_bounds : forall G x T1 T2 A,
+    inert G ->
+    ty_trm ty_precise sub_general G (trm_var (avar_f x)) (typ_rcd (dec_typ A T1 T1)) ->
+    ty_trm ty_precise sub_general G (trm_var (avar_f x)) (typ_rcd (dec_typ A T2 T2)) ->
+    T1 = T2.
+Proof.
+  introv Hi H1 H2.
+  destruct (precise_flow_lemma H1) as [T1' Pf1].
+  destruct (precise_flow_lemma H2) as [T2' Pf2].
+  lets Heq: (x_bound_unique Hi Pf1 Pf2). subst.
+  apply* pf_inert_unique_tight_bounds.
 Qed.
 
 Lemma inert_ok : forall G,
@@ -203,4 +392,34 @@ Proof.
   inversions HG. false* empty_push_inv.
   destruct (eq_push_inv H) as [Hx [HT HG]]. subst.
   apply* ok_push.
+Qed.
+
+Lemma pf_dec_typ_inv : forall G x T A S U,
+    inert G ->
+    precise_flow x G T (typ_rcd (dec_typ A S U)) ->
+    S = U.
+Proof.
+  introv Hi Pf. destruct (pf_inert_rcd_U Hi Pf) as [V H]. subst.
+  destruct (pf_inert_or_rcd Hi Pf) as [H1 | H1]; inversions H1. inversions H.
+  inversions* H1.
+Qed.
+
+Lemma precise_dec_typ_inv : forall G x A S U,
+    inert G ->
+    ty_trm ty_precise sub_general G (trm_var (avar_f x)) (typ_rcd (dec_typ A S U)) ->
+    S = U.
+Proof.
+  introv Hi Hpt. destruct (precise_flow_lemma Hpt) as [V Pf].
+  apply* pf_dec_typ_inv.
+Qed.
+
+Lemma inert_precise_all_inv : forall x G S T,
+    inert G ->
+    ty_trm ty_precise sub_general G (trm_var (avar_f x)) (typ_all S T) ->
+    binds x (typ_all S T) G.
+Proof.
+  introv Hgd Htyp.
+  destruct (precise_flow_lemma Htyp) as [V Pf].
+  pose proof (pf_inert_lambda_U Hgd Pf) as H. subst.
+  apply* pf_binds.
 Qed.
